\chapter{Functions Properties}
$$f: X \to Y \quad A \subseteq X, B \subseteq Y$$
\begin{definition}[Image]
	$f(A) = \{ y \in Y \mid \exists x \in A \text{ s.t. } f(x)=y \}$
\end{definition}
\begin{definition}[Inverse Image]
	$f^{-1}(B) = \{ x \in X \mid f(x) \in B \}$
\end{definition}
\begin{definition}[Fiber]
	Fiber of $y$ is inverse image of $\{y\}$.
\end{definition}
\begin{definition}[Well definedness]
	$\forall x \in X, \exists ! y \in Y \text{ s.t. } f(x) = y$\\
	%	-- or --\\
	%	$\forall x \in X, \exists y \in Y \text{ s.t. } f(x) = y$\\
	%	$\forall y,y' \in Y, y \neq y', f^{-1}(y) \cap f^{-1}(y') = \emptyset$
\end{definition}
\begin{definition}[Injectivity]
	$\forall x,x' \in X, x \neq x', f(x) \neq f(x')$
\end{definition}
\begin{definition}[Surjectivity]
	$\forall y \in Y, \exists x \in X \text{ s.t. } f(x) = y$
\end{definition}
\begin{definition}[Bijectivity]
	Injectivity plus Surjectivity:
	$\forall y \in Y, \exists! x \in X \text{ s.t. } f(x) = y$
\end{definition}
\begin{definition}[Invertibility]
	$f^{-1}: Y \to X$ well defined.
\end{definition}
\begin{remark}[Alternative Definition of Inverse]
	$f \circ f^{-1} = Id \mid_X$  and $f^{-1} \circ f = Id \mid_Y$
\end{remark}
\begin{remark}[Invertibility and Bijectivity]
	$f$ bijective $\iff$ $f$ invertible.
\end{remark}
\begin{remark}[Inverse is Invertible]
	$f^{-1}$ is invertible, and $(f^{-1})^{-1}=f$.
\end{remark}
\begin{property}[Injections between finite intervals]
	$m,n \in \N^*$, there exists an injection $f:\llbracket 1;m \rrbracket \rightarrow \llbracket 1;n \rrbracket$ if and only if $m \leq n$.
\end{property}
\begin{proof}
	By induction on $m$, carefully checking $m \leq n$.
\end{proof}
\begin{property}[Bijections between finite intervals]
	$n,m \in \N^*$, there exists a bijection $f:\llbracket 1;m \rrbracket \rightarrow \llbracket 1;n \rrbracket$ if and only if $m=n$.
\end{property}
\begin{proof}
	Use last property \& inverse.
\end{proof}
\begin{property}[Compositions]
	Composition preserve injectivity/surjectivity/bijectivity/invertibility:
	$f: X \to Y, \ g: Y \to Z \text{ injectives } \implies f \circ g \text{ is injective}$\\
	$f: X \to Y, \ g: Y \to Z \text{ surjectives } \implies f \circ g \text{ is surjective}$\\
	$f: X \to Y, \ g: Y \to Z \text{ bijections/invertibles } \implies f \circ g \text{ is bijective/invertible}$
\end{property}
\begin{proof}
	Trivial
\end{proof}
\begin{property}
	An injection between two sets of the same size is bijective.
\end{property}
\begin{proof}
	By contradiction.
\end{proof}

